src/finite_map/alistScript.sml
@@ -404,7 +404,8 @@ metis_tac[PERM_TRANS,PERM_SYM,ALL_DISTINCT_PERM,PERM_MAP,alist_to_fmap_to_alist_
 local open pairTheory boolSimps sortingTheory relationTheory in
 
 val ALOOKUP_ALL_DISTINCT_EL = store_thm("ALOOKUP_ALL_DISTINCT_EL",
-  ``∀ls n. n < LENGTH ls ∧ ALL_DISTINCT (MAP FST ls) ⇒ (ALOOKUP ls (FST (EL n ls)) = SOME (SND (EL n ls)))``,
+  ``!ls n. n < LENGTH ls /\ ALL_DISTINCT (MAP FST ls) ==>
+           (ALOOKUP ls (FST (EL n ls)) = SOME (SND (EL n ls)))``,
   Induct >> simp[] >>
   Cases >> simp[] >>
   Cases >> simp[] >>
@@ -412,21 +413,24 @@ val ALOOKUP_ALL_DISTINCT_EL = store_thm("ALOOKUP_ALL_DISTINCT_EL",
   metis_tac[MEM_EL])
 
 val ALOOKUP_ZIP_MAP_SND = store_thm("ALOOKUP_ZIP_MAP_SND",
-  ``∀l1 l2 k f. (LENGTH l1 = LENGTH l2) ⇒
+  ``!l1 l2 k f.
+      (LENGTH l1 = LENGTH l2) ==>
       (ALOOKUP (ZIP(l1,MAP f l2)) = OPTION_MAP f o (ALOOKUP (ZIP(l1,l2))))``,
   Induct >> simp[LENGTH_NIL,LENGTH_NIL_SYM,FUN_EQ_THM] >>
   gen_tac >> Cases >> simp[] >> rw[] >> rw[])
 
 val ALOOKUP_FILTER = store_thm("ALOOKUP_FILTER",
-  ``∀ls x. ALOOKUP (FILTER (λ(k,v). P k) ls) x =
+  ``!ls x. ALOOKUP (FILTER (\(k,v). P k) ls) x =
            if P x then ALOOKUP ls x else NONE``,
   Induct >> simp[] >> Cases >> simp[] >> rw[] >> fs[] >> metis_tac[])
 
 val ALOOKUP_APPEND_same = store_thm("ALOOKUP_APPEND_same",
-  ``∀l1 l2 l. (ALOOKUP l1 = ALOOKUP l2) ==> (ALOOKUP (l1 ++ l) = ALOOKUP (l2 ++ l))``,
+  ``!l1 l2 l.
+      (ALOOKUP l1 = ALOOKUP l2) ==> (ALOOKUP (l1 ++ l) = ALOOKUP (l2 ++ l))``,
   rw[ALOOKUP_APPEND,FUN_EQ_THM])
+
 val ALOOKUP_IN_FRANGE = store_thm("ALOOKUP_IN_FRANGE",
-  ``∀ls k v. (ALOOKUP ls k = SOME v) ⇒ v ∈ FRANGE (alist_to_fmap ls)``,
+  ``!ls k v. (ALOOKUP ls k = SOME v) ==> v IN FRANGE (alist_to_fmap ls)``,
   Induct >> simp[] >> Cases >> simp[] >> rw[] >>
   simp[IN_FRANGE,DOMSUB_FAPPLY_THM] >>
   full_simp_tac std_ss [Once(SYM (CONJUNCT1 ALOOKUP_EQ_FLOOKUP)),FLOOKUP_DEF] >>
@@ -434,7 +438,7 @@ val ALOOKUP_IN_FRANGE = store_thm("ALOOKUP_IN_FRANGE",
 
 val FRANGE_alist_to_fmap_SUBSET = store_thm(
 "FRANGE_alist_to_fmap_SUBSET",
-``FRANGE (alist_to_fmap ls) ⊆ IMAGE SND (set ls)``,
+``FRANGE (alist_to_fmap ls) SUBSET IMAGE SND (set ls)``,
 srw_tac[DNF_ss][FRANGE_DEF,SUBSET_DEF,pairTheory.EXISTS_PROD] >>
 qmatch_assum_rename_tac `MEM z (MAP FST ls)`[] >>
 qexists_tac `z` >>
@@ -443,7 +447,8 @@ rw[])
 
 val IN_FRANGE_alist_to_fmap_suff = store_thm(
 "IN_FRANGE_alist_to_fmap_suff",
-``(∀v. MEM v (MAP SND ls) ⇒ P v) ⇒ (∀v. v ∈ FRANGE (alist_to_fmap ls) ⇒ P v)``,
+``(!v. MEM v (MAP SND ls) ==> P v) ==>
+  (!v. v IN FRANGE (alist_to_fmap ls) ==> P v)``,
 rw[] >>
 imp_res_tac(SIMP_RULE(srw_ss())[SUBSET_DEF]FRANGE_alist_to_fmap_SUBSET) >>
 fs[MEM_MAP] >>
@@ -451,32 +456,32 @@ PROVE_TAC[])
 
 val alist_to_fmap_MAP_matchable = store_thm(
 "alist_to_fmap_MAP_matchable",
-``∀f1 f2 al mal v. INJ f1 (set (MAP FST al)) UNIV ∧
-  (mal = MAP (λ(x,y). (f1 x,f2 y)) al) ∧
-  (v = MAP_KEYS f1 (f2 o_f alist_to_fmap al)) ⇒
+``!f1 f2 al mal v. INJ f1 (set (MAP FST al)) UNIV /\
+  (mal = MAP (\(x,y). (f1 x,f2 y)) al) /\
+  (v = MAP_KEYS f1 (f2 o_f alist_to_fmap al)) ==>
   (alist_to_fmap mal = v)``,
 METIS_TAC[alist_to_fmap_MAP])
 
 val MAP_values_fmap_to_alist = store_thm(
 "MAP_values_fmap_to_alist",
-``∀f fm. MAP (λ(k,v). (k, f v)) (fmap_to_alist fm) = fmap_to_alist (f o_f fm)``,
+``!f fm. MAP (\(k,v). (k, f v)) (fmap_to_alist fm) = fmap_to_alist (f o_f fm)``,
 rw[fmap_to_alist_def,MAP_MAP_o,MAP_EQ_f])
 
 val INJ_I = prove (
-``∀s t. INJ I s t ⇔ s ⊆ t``,
+``!s t. INJ I s t <=> s SUBSET t``,
 SRW_TAC[][INJ_DEF,SUBSET_DEF])
 
 val MAP_KEYS_I = store_thm(
 "MAP_KEYS_I",
-``∀fm. MAP_KEYS I fm = fm``,
+``!fm. MAP_KEYS I fm = fm``,
 rw[GSYM fmap_EQ_THM,MAP_KEYS_def,EXTENSION] >>
 metis_tac[MAP_KEYS_def,INJ_I,SUBSET_UNIV,combinTheory.I_THM])
 
 val alist_to_fmap_MAP_values = store_thm(
 "alist_to_fmap_MAP_values",
-``∀f al. alist_to_fmap (MAP (λ(k,v). (k, f v)) al) = f o_f (alist_to_fmap al)``,
+``!f al. alist_to_fmap (MAP (\(k,v). (k, f v)) al) = f o_f (alist_to_fmap al)``,
 rw[] >>
-Q.ISPECL_THEN [`I:γ->γ`,`f`,`al`] match_mp_tac alist_to_fmap_MAP_matchable >>
+Q.ISPECL_THEN [`I:'c->'c`,`f`,`al`] match_mp_tac alist_to_fmap_MAP_matchable >>
 SRW_TAC[][INJ_DEF,SUBSET_DEF,MAP_KEYS_I])
 
 val set_MAP_FST_fmap_to_alist = store_thm(
@@ -485,7 +490,7 @@ val set_MAP_FST_fmap_to_alist = store_thm(
 METIS_TAC[fmap_to_alist_to_fmap,FDOM_alist_to_fmap])
 
 val alookup_distinct_reverse = Q.store_thm ("alookup_distinct_reverse",
-`!l k. ALL_DISTINCT (MAP FST l) ⇒ (ALOOKUP (REVERSE l) k = ALOOKUP l k)`,
+`!l k. ALL_DISTINCT (MAP FST l) ==> (ALOOKUP (REVERSE l) k = ALOOKUP l k)`,
  Induct_on `l` >>
  rw [] >>
  PairCases_on `h` >>
@@ -519,7 +524,7 @@ val flookup_fupdate_list = Q.store_thm ("flookup_fupdate_list",
 val fupdate_list_funion = store_thm("fupdate_list_funion",
 ``!m l. m|++l = FUNION (FEMPTY |++l) m``,
  Induct_on `l`
- >- rw [FUPDATE_LIST, FUNION_FEMPTY_1] >> 
+ >- rw [FUPDATE_LIST, FUNION_FEMPTY_1] >>
  REWRITE_TAC [FUPDATE_LIST_THM] >>
  rpt GEN_TAC >>
  pop_assum (qspecl_then [`m|+h`] mp_tac) >>
@@ -532,7 +537,7 @@ val fupdate_list_funion = store_thm("fupdate_list_funion",
  fs []);
 
 val mem_to_flookup = Q.store_thm ("mem_to_flookup",
-`!x y l. ALL_DISTINCT (MAP FST l) ∧ MEM (x,y) l ⇒ (FLOOKUP (FEMPTY |++ l) x = SOME y)`,
+`!x y l. ALL_DISTINCT (MAP FST l) /\ MEM (x,y) l ==> (FLOOKUP (FEMPTY |++ l) x = SOME y)`,
  Induct_on `l` >>
  rw [] >>
  fs [flookup_fupdate_list] >>
@@ -550,7 +555,7 @@ val mem_to_flookup = Q.store_thm ("mem_to_flookup",
  metis_tac [FST]);
 
 val alookup_filter = Q.store_thm ("alookup_filter",
-`!f l x. ALOOKUP l x = ALOOKUP (FILTER (λ(x',y). x = x') l) x`,
+`!f l x. ALOOKUP l x = ALOOKUP (FILTER (\(x',y). x = x') l) x`,
  Induct_on `l` >>
  rw [ALOOKUP_def] >>
  PairCases_on `h` >>
@@ -563,16 +568,16 @@ alist_range m = { v | ?k. ALOOKUP m k = SOME v }`;
 
 val alookup_stable_sorted = Q.store_thm ("alookup_stable_sorted",
 `!R sort x l.
-  transitive R ∧ total R ∧
+  transitive R /\ total R /\
   STABLE sort (inv_image R FST)
-  ⇒
+  ==>
   (ALOOKUP (sort (inv_image R FST) l) x = ALOOKUP l x)`,
  rw [] >>
  ONCE_REWRITE_TAC [alookup_filter] >>
  fs [STABLE_DEF, SORTS_DEF] >>
- pop_assum (mp_tac o GSYM o Q.SPEC `(λ(x',y). x = x')`) >>
+ pop_assum (mp_tac o GSYM o Q.SPEC `(\(x',y). x = x')`) >>
  rw [] >>
- match_mp_tac (METIS_PROVE [] ``(x = x') ⇒ (f x y = f x' y)``) >> 
+ match_mp_tac (METIS_PROVE [] ``(x = x') ==> (f x y = f x' y)``) >>
  pop_assum match_mp_tac >>
  rw [] >>
  PairCases_on `x'` >>
@@ -581,7 +586,8 @@ val alookup_stable_sorted = Q.store_thm ("alookup_stable_sorted",
  metis_tac []);
 
 val ALOOKUP_ALL_DISTINCT_PERM_same = store_thm("ALOOKUP_ALL_DISTINCT_PERM_same",
-  ``∀l1 l2. ALL_DISTINCT (MAP FST l1) ∧ PERM (MAP FST l1) (MAP FST l2) ∧ (set l1 = set l2) ⇒ (ALOOKUP l1 = ALOOKUP l2)``,
+  ``!l1 l2. ALL_DISTINCT (MAP FST l1) /\ PERM (MAP FST l1) (MAP FST l2) /\
+            (set l1 = set l2) ==> (ALOOKUP l1 = ALOOKUP l2)``,
   simp[EXTENSION] >>
   rw[FUN_EQ_THM] >>
   Cases_on`ALOOKUP l2 x` >- (
