src/finite_map/finite_mapScript.sml
@@ -176,7 +176,6 @@ val update_rep = Term`\(f:'a->'b+one) x y. \a. if a=x then INL y else f a`;
 val empty_rep = Term`(\a. INR one):'a -> 'b + one`;
 
 
-
 (*---------------------------------------------------------------------------
       Now some theorems
  --------------------------------------------------------------------------- *)
@@ -1827,8 +1826,6 @@ val _ =
    "FLOOKUP_UPDATE"];
 
 
-
-
 (*---------------------------------------------------------------------------*)
 (* Mapping for finite maps with two arguments, compare to o_f                *)
 (* added 17 March 2009 by Thomas Tuerk, updated 26 March                     *)
@@ -2254,17 +2251,17 @@ val fmap_size_def =
 (* Various lemmas from the CakeML project https://cakeml.org                 *)
 (*---------------------------------------------------------------------------*)
 
-local 
-  open lcsymtacs optionTheory rich_listTheory listTheory boolSimps sortingTheory 
+local
+  open lcsymtacs optionTheory rich_listTheory listTheory boolSimps sortingTheory
 in
 
 val o_f_FUNION = store_thm("o_f_FUNION",
-  ``f o_f (f1 ⊌ f2) = (f o_f f1) ⊌ (f o_f f2)``,
+  ``f o_f (FUNION f1 f2) = FUNION (f o_f f1) (f o_f f2)``,
   simp[GSYM fmap_EQ_THM,FUNION_DEF] >>
   rw[o_f_FAPPLY]);
 
 val FDOM_FOLDR_DOMSUB = store_thm("FDOM_FOLDR_DOMSUB",
-  ``∀ls fm. FDOM (FOLDR (λk m. m \\ k) fm ls) = FDOM fm DIFF set ls``,
+  ``!ls fm. FDOM (FOLDR (\k m. m \\ k) fm ls) = FDOM fm DIFF set ls``,
   Induct >> simp[] >>
   ONCE_REWRITE_TAC[EXTENSION] >>
   simp[] >> metis_tac[]);
@@ -2274,7 +2271,7 @@ val FEVERY_SUBMAP = store_thm("FEVERY_SUBMAP",
   SRW_TAC[][FEVERY_DEF,SUBMAP_DEF]);
 
 val FEVERY_ALL_FLOOKUP = store_thm("FEVERY_ALL_FLOOKUP",
-  ``∀P f. FEVERY P f ⇔ ∀k v. (FLOOKUP f k = SOME v) ⇒ P (k,v)``,
+  ``!P f. FEVERY P f <=> !k v. (FLOOKUP f k = SOME v) ==> P (k,v)``,
   SRW_TAC[][FEVERY_DEF,FLOOKUP_DEF]);
 
 val FUPDATE_LIST_CANCEL = store_thm("FUPDATE_LIST_CANCEL",
@@ -2287,19 +2284,20 @@ val FUPDATE_LIST_CANCEL = store_thm("FUPDATE_LIST_CANCEL",
   FULL_SIMP_TAC(srw_ss())[]);
 
 val FUPDATE_EQ_FUNION = store_thm("FUPDATE_EQ_FUNION",
-  ``∀fm kv. fm |+ kv = (FEMPTY |+ kv) ⊌ fm``,
+  ``!fm kv. fm |+ kv = FUNION (FEMPTY |+ kv) fm``,
   gen_tac >> Cases >>
   simp[GSYM fmap_EQ_THM,FDOM_FUPDATE,FAPPLY_FUPDATE_THM,FUNION_DEF] >>
   simp[EXTENSION]);
 
 val FUPDATE_LIST_APPEND_COMMUTES = store_thm("FUPDATE_LIST_APPEND_COMMUTES",
-  ``!l1 l2 fm. DISJOINT (set (MAP FST l1)) (set (MAP FST l2)) ⇒ (fm |++ l1 |++ l2 = fm |++ l2 |++ l1)``,
+  ``!l1 l2 fm. DISJOINT (set (MAP FST l1)) (set (MAP FST l2)) ==>
+               (fm |++ l1 |++ l2 = fm |++ l2 |++ l1)``,
   Induct >- rw[FUPDATE_LIST_THM] >>
   Cases >> rw[FUPDATE_LIST_THM] >>
   metis_tac[FUPDATE_FUPDATE_LIST_COMMUTES]);
 
 val fmap_rel_OPTREL_FLOOKUP = store_thm("fmap_rel_OPTREL_FLOOKUP",
-  ``fmap_rel R f1 f2 = ∀k. OPTREL R (FLOOKUP f1 k) (FLOOKUP f2 k)``,
+  ``fmap_rel R f1 f2 = !k. OPTREL R (FLOOKUP f1 k) (FLOOKUP f2 k)``,
   rw[fmap_rel_def,optionTheory.OPTREL_def,FLOOKUP_DEF,EXTENSION] >>
   PROVE_TAC[]);
 
@@ -2318,7 +2316,8 @@ val FUPDATE_LIST_ALL_DISTINCT_PERM = store_thm("FUPDATE_LIST_ALL_DISTINCT_PERM",
   qexists_tac `(fm |++ (M ++ N)) |+ (h0,h1)` >>
   conj_tac >- metis_tac[sortingTheory.ALL_DISTINCT_PERM,sortingTheory.PERM_MAP] >>
   rw[FUPDATE_LIST_APPEND] >>
-  `h0 ∉ set (MAP FST N)` by metis_tac[sortingTheory.PERM_MEM_EQ,MEM_MAP,MEM_APPEND] >>
+  `h0 NOTIN set (MAP FST N)`
+  by metis_tac[sortingTheory.PERM_MEM_EQ,MEM_MAP,MEM_APPEND] >>
   imp_res_tac FUPDATE_FUPDATE_LIST_COMMUTES >>
   rw[FUPDATE_LIST_THM]);
 
@@ -2351,8 +2350,9 @@ val DRESTRICT_DOMSUB = store_thm("DRESTRICT_DOMSUB",
   SRW_TAC[][DRESTRICT_DEF]);
 
 val DRESTRICT_SUBSET_SUBMAP_gen = store_thm("DRESTRICT_SUBSET_SUBMAP_gen",
-  ``!f1 f2 s t. DRESTRICT f1 s ⊑ DRESTRICT f2 s ∧ t ⊆ s
-    ==> DRESTRICT f1 t ⊑ DRESTRICT f2 t``,
+  ``!f1 f2 s t.
+     DRESTRICT f1 s SUBMAP DRESTRICT f2 s /\ t SUBSET s ==>
+     DRESTRICT f1 t SUBMAP DRESTRICT f2 t``,
   rw[SUBMAP_DEF,DRESTRICT_DEF,SUBSET_DEF])
 
 
@@ -2361,7 +2361,7 @@ val DRESTRICT_FUNION_SAME = store_thm("DRESTRICT_FUNION_SAME",
   SRW_TAC[][GSYM SUBMAP_FUNION_ABSORPTION])
 
 val DRESTRICT_EQ_DRESTRICT_SAME = store_thm("DRESTRICT_EQ_DRESTRICT_SAME",
-  ``(DRESTRICT f1 s = DRESTRICT f2 s) ⇔
+  ``(DRESTRICT f1 s = DRESTRICT f2 s) <=>
     (s INTER FDOM f1 = s INTER FDOM f2) /\
     (!x. x IN FDOM f1 /\ x IN s ==> (f1 ' x = f2 ' x))``,
   SRW_TAC[][DRESTRICT_EQ_DRESTRICT,SUBMAP_DEF,DRESTRICT_DEF,EXTENSION] THEN
@@ -2369,8 +2369,8 @@ val DRESTRICT_EQ_DRESTRICT_SAME = store_thm("DRESTRICT_EQ_DRESTRICT_SAME",
 
 val FOLDL2_FUPDATE_LIST = store_thm(
 "FOLDL2_FUPDATE_LIST",
-``!f1 f2 bs cs a. (LENGTH bs = LENGTH cs) ⇒
-  (FOLDL2 (λfm b c. fm |+ (f1 b c, f2 b c)) a bs cs =
+``!f1 f2 bs cs a. (LENGTH bs = LENGTH cs) ==>
+  (FOLDL2 (\fm b c. fm |+ (f1 b c, f2 b c)) a bs cs =
    a |++ ZIP (MAP2 f1 bs cs, MAP2 f2 bs cs))``,
 SRW_TAC[][FUPDATE_LIST,FOLDL2_FOLDL,MAP2_MAP,ZIP_MAP,MAP_ZIP,
           rich_listTheory.FOLDL_MAP,rich_listTheory.LENGTH_MAP2,
@@ -2378,17 +2378,18 @@ SRW_TAC[][FUPDATE_LIST,FOLDL2_FOLDL,MAP2_MAP,ZIP_MAP,MAP_ZIP,
 
 val FOLDL2_FUPDATE_LIST_paired = store_thm(
 "FOLDL2_FUPDATE_LIST_paired",
-``!f1 f2 bs cs a. (LENGTH bs = LENGTH cs) ⇒
-  (FOLDL2 (λfm b (c,d). fm |+ (f1 b c d, f2 b c d)) a bs cs =
-   a |++ ZIP (MAP2 (λb. UNCURRY (f1 b)) bs cs, MAP2 (λb. UNCURRY (f2 b)) bs cs))``,
+``!f1 f2 bs cs a. (LENGTH bs = LENGTH cs) ==>
+  (FOLDL2 (\fm b (c,d). fm |+ (f1 b c d, f2 b c d)) a bs cs =
+   a |++ ZIP (MAP2 (\b. UNCURRY (f1 b)) bs cs, MAP2 (\b. UNCURRY (f2 b)) bs cs))``,
 rw[FOLDL2_FOLDL,MAP2_MAP,ZIP_MAP,MAP_ZIP,LENGTH_ZIP,
    pairTheory.UNCURRY,pairTheory.LAMBDA_PROD,FUPDATE_LIST,
    rich_listTheory.FOLDL_MAP])
 
 val DRESTRICT_FUNION_SUBSET = store_thm("DRESTRICT_FUNION_SUBSET",
-  ``s2 ⊆ s1 ⇒ ∃h. (DRESTRICT f s1 ⊌ g = DRESTRICT f s2 ⊌ h)``,
+  ``s2 SUBSET s1 ==>
+    ?h. (FUNION (DRESTRICT f s1) g = FUNION (DRESTRICT f s2) h)``,
   strip_tac >>
-  qexists_tac `DRESTRICT f s1 ⊌ g` >>
+  qexists_tac `FUNION (DRESTRICT f s1) g` >>
   match_mp_tac EQ_SYM >>
   REWRITE_TAC[GSYM SUBMAP_FUNION_ABSORPTION] >>
   rw[SUBMAP_DEF,DRESTRICT_DEF,FUNION_DEF] >>
@@ -2401,11 +2402,11 @@ PROVE_TAC[FUPDATE_LIST_APPLY_NOT_MEM])
 
 val FUPDATE_LIST_APPLY_HO_THM = store_thm(
 "FUPDATE_LIST_APPLY_HO_THM",
-``∀P f kvl k.
-(∃n. n < LENGTH kvl ∧ (k = EL n (MAP FST kvl)) ∧ P (EL n (MAP SND kvl)) ∧
-     (∀m. n < m ∧ m < LENGTH kvl ⇒ EL m (MAP FST kvl) ≠ k)) ∨
-(¬MEM k (MAP FST kvl) ∧ P (f ' k))
-⇒ (P ((f |++ kvl) ' k))``,
+``!P f kvl k.
+(?n. n < LENGTH kvl /\ (k = EL n (MAP FST kvl)) /\ P (EL n (MAP SND kvl)) /\
+     (!m. n < m /\ m < LENGTH kvl ==> EL m (MAP FST kvl) <> k)) \/
+(~MEM k (MAP FST kvl) /\ P (f ' k))
+==> (P ((f |++ kvl) ' k))``,
 metis_tac[FUPDATE_LIST_APPLY_MEM,FUPDATE_LIST_APPLY_NOT_MEM])
 
 val FUPDATE_SAME_APPLY = store_thm(
@@ -2428,9 +2429,9 @@ PROVE_TAC[])
 
 val FUPDATE_LIST_ALL_DISTINCT_APPLY_MEM = store_thm(
 "FUPDATE_LIST_ALL_DISTINCT_APPLY_MEM",
-``!P ls k v fm. ALL_DISTINCT (MAP FST ls) ∧
-  MEM (k,v) ls ∧
-  P v ⇒
+``!P ls k v fm. ALL_DISTINCT (MAP FST ls) /\
+  MEM (k,v) ls /\
+  P v ==>
   P ((fm |++ ls) ' k)``,
 rw[] >>
 ho_match_mp_tac FUPDATE_LIST_APPLY_HO_THM >>
@@ -2443,7 +2444,7 @@ rw[EL_MAP] >> spose_not_then strip_assume_tac >>
 rw[] >> fs[])
 
 val FUPDATE_LIST_ALL_DISTINCT_REVERSE = store_thm("FUPDATE_LIST_ALL_DISTINCT_REVERSE",
-  ``∀ls. ALL_DISTINCT (MAP FST ls) ⇒ ∀fm. fm |++ (REVERSE ls) = fm |++ ls``,
+  ``!ls. ALL_DISTINCT (MAP FST ls) ==> !fm. fm |++ (REVERSE ls) = fm |++ ls``,
   Induct >- rw[] >>
   qx_gen_tac `p` >> PairCases_on `p` >>
   rw[FUPDATE_LIST_APPEND,FUPDATE_LIST_THM] >>
@@ -2454,16 +2455,16 @@ val FUPDATE_LIST_ALL_DISTINCT_REVERSE = store_thm("FUPDATE_LIST_ALL_DISTINCT_REV
 
 val IN_FRANGE = store_thm(
 "IN_FRANGE",
-``!f v. v IN FRANGE f ⇔ ?k. k IN FDOM f /\ (f ' k = v)``,
+``!f v. v IN FRANGE f <=> ?k. k IN FDOM f /\ (f ' k = v)``,
 SRW_TAC[][FRANGE_DEF])
 
 val IN_FRANGE_FLOOKUP = store_thm("IN_FRANGE_FLOOKUP",
-``!f v. v IN FRANGE f ⇔ ∃k. FLOOKUP f k = SOME v``,
+``!f v. v IN FRANGE f <=> ?k. FLOOKUP f k = SOME v``,
 rw[IN_FRANGE,FLOOKUP_DEF])
 
 val FRANGE_FUPDATE_LIST_SUBSET = store_thm(
 "FRANGE_FUPDATE_LIST_SUBSET",
-``∀ls fm. FRANGE (fm |++ ls) ⊆ FRANGE fm ∪ (set (MAP SND ls))``,
+``!ls fm. FRANGE (fm |++ ls) SUBSET FRANGE fm UNION (set (MAP SND ls))``,
 Induct >- rw[FUPDATE_LIST_THM] >>
 qx_gen_tac `p` >> qx_gen_tac `fm` >>
 pop_assum (qspec_then `fm |+ p` mp_tac) >>
@@ -2477,69 +2478,69 @@ PROVE_TAC[])
 
 val IN_FRANGE_FUPDATE_LIST_suff = store_thm(
 "IN_FRANGE_FUPDATE_LIST_suff",
-``(∀v. v ∈ FRANGE fm ⇒ P v) ∧ (∀v. MEM v (MAP SND ls) ⇒ P v) ⇒
-    ∀v. v ∈ FRANGE (fm |++ ls) ⇒ P v``,
+``(!v. v IN FRANGE fm ==> P v) /\ (!v. MEM v (MAP SND ls) ==> P v) ==>
+    !v. v IN FRANGE (fm |++ ls) ==> P v``,
 rw[] >>
 imp_res_tac(SIMP_RULE(srw_ss())[SUBSET_DEF]FRANGE_FUPDATE_LIST_SUBSET) >>
 PROVE_TAC[])
 
 val FRANGE_FUNION_SUBSET = store_thm(
 "FRANGE_FUNION_SUBSET",
-``FRANGE (f1 ⊌ f2) ⊆ FRANGE f1 ∪ FRANGE f2``,
+``FRANGE (FUNION f1 f2) SUBSET FRANGE f1 UNION FRANGE f2``,
 srw_tac[DNF_ss][FRANGE_DEF,SUBSET_DEF,FUNION_DEF] >>
 PROVE_TAC[])
 
 val IN_FRANGE_FUNION_suff = store_thm(
 "IN_FRANGE_FUNION_suff",
-``(∀v. v ∈ FRANGE f1 ⇒ P v) ∧ (∀v. v ∈ FRANGE f2 ⇒ P v) ⇒
-  (∀v. v ∈ FRANGE (f1 ⊌ f2) ⇒ P v)``,
+``(!v. v IN FRANGE f1 ==> P v) /\ (!v. v IN FRANGE f2 ==> P v) ==>
+  (!v. v IN FRANGE (FUNION f1 f2) ==> P v)``,
 rw[] >>
 imp_res_tac(SIMP_RULE(srw_ss())[SUBSET_DEF]FRANGE_FUNION_SUBSET) >>
 PROVE_TAC[])
 
 val FRANGE_DOMSUB_SUBSET = store_thm(
 "FRANGE_DOMSUB_SUBSET",
-``FRANGE (fm \\ k) ⊆ FRANGE fm``,
+``FRANGE (fm \\ k) SUBSET FRANGE fm``,
 srw_tac[DNF_ss][FRANGE_DEF,SUBSET_DEF,DOMSUB_FAPPLY_THM] >>
 PROVE_TAC[])
 
 val IN_FRANGE_DOMSUB_suff = store_thm(
 "IN_FRANGE_DOMSUB_suff",
-``(∀v. v ∈ FRANGE fm ⇒ P v) ⇒ (∀v. v ∈ FRANGE (fm \\ k) ⇒ P v)``,
+``(!v. v IN FRANGE fm ==> P v) ==> (!v. v IN FRANGE (fm \\ k) ==> P v)``,
 rw[] >>
 imp_res_tac(SIMP_RULE(srw_ss())[SUBSET_DEF]FRANGE_DOMSUB_SUBSET) >>
 PROVE_TAC[])
 
 val FRANGE_DRESTRICT_SUBSET = store_thm(
 "FRANGE_DRESTRICT_SUBSET",
-``FRANGE (DRESTRICT fm s) ⊆ FRANGE fm``,
+``FRANGE (DRESTRICT fm s) SUBSET FRANGE fm``,
 srw_tac[DNF_ss][FRANGE_DEF,SUBSET_DEF,DRESTRICT_DEF] >>
 PROVE_TAC[])
 
 val IN_FRANGE_DRESTRICT_suff = store_thm(
 "IN_FRANGE_DRESTRICT_suff",
-``(∀v. v ∈ FRANGE fm ⇒ P v) ⇒ (∀v. v ∈ FRANGE (DRESTRICT fm s) ⇒ P v)``,
+``(!v. v IN FRANGE fm ==> P v) ==> (!v. v IN FRANGE (DRESTRICT fm s) ==> P v)``,
 rw[] >>
 imp_res_tac(SIMP_RULE(srw_ss())[SUBSET_DEF]FRANGE_DRESTRICT_SUBSET) >>
 PROVE_TAC[])
 
 val FRANGE_FUPDATE_SUBSET = store_thm(
 "FRANGE_FUPDATE_SUBSET",
-``FRANGE (fm |+ kv) ⊆ FRANGE fm ∪ {SND kv}``,
+``FRANGE (fm |+ kv) SUBSET FRANGE fm UNION {SND kv}``,
 Cases_on `kv` >>
 rw[FRANGE_DEF,SUBSET_DEF,DOMSUB_FAPPLY_THM] >>
 rw[] >> PROVE_TAC[])
 
 val IN_FRANGE_FUPDATE_suff = store_thm(
 "IN_FRANGE_FUPDATE_suff",
-`` (∀v. v ∈ FRANGE fm ⇒ P v) ∧ (P (SND kv))
-⇒ (∀v. v ∈ FRANGE (fm |+ kv) ⇒ P v)``,
+`` (!v. v IN FRANGE fm ==> P v) /\ (P (SND kv))
+==> (!v. v IN FRANGE (fm |+ kv) ==> P v)``,
 rw[] >>
 imp_res_tac(SIMP_RULE(srw_ss())[SUBSET_DEF]FRANGE_FUPDATE_SUBSET) >>
 fs[])
 
 val IN_FRANGE_o_f_suff = store_thm("IN_FRANGE_o_f_suff",
-  ``(∀v. v ∈ FRANGE fm ⇒ P (f v)) ⇒ ∀v. v ∈ FRANGE (f o_f fm) ⇒ P v``,
+  ``(!v. v IN FRANGE fm ==> P (f v)) ==> !v. v IN FRANGE (f o_f fm) ==> P v``,
   rw[IN_FRANGE] >> rw[] >> first_x_assum match_mp_tac >> PROVE_TAC[])
 
 (* DRESTRICT stuff *)
@@ -2556,13 +2557,13 @@ SRW_TAC[][SUBMAP_DEF,SUBSET_DEF,DRESTRICT_DEF])
 
 val DRESTRICTED_FUNION = store_thm(
 "DRESTRICTED_FUNION",
-``∀f1 f2 s. DRESTRICT (f1 ⊌ f2) s = DRESTRICT f1 s ⊌ DRESTRICT f2 (s DIFF FDOM f1)``,
+``!f1 f2 s. DRESTRICT (FUNION f1 f2) s = FUNION (DRESTRICT f1 s) (DRESTRICT f2 (s DIFF FDOM f1))``,
 rw[GSYM fmap_EQ_THM,DRESTRICT_DEF,FUNION_DEF] >> rw[] >>
 rw[EXTENSION] >> PROVE_TAC[])
 
 val FRANGE_DRESTRICT_SUBSET = store_thm(
 "FRANGE_DRESTRICT_SUBSET",
-``FRANGE (DRESTRICT fm s) ⊆ FRANGE fm``,
+``FRANGE (DRESTRICT fm s) SUBSET FRANGE fm``,
 SRW_TAC[][FRANGE_DEF,SUBSET_DEF,DRESTRICT_DEF] THEN
 SRW_TAC[][] THEN PROVE_TAC[])
 
@@ -2572,8 +2573,8 @@ val DRESTRICT_FDOM = store_thm(
 SRW_TAC[][GSYM fmap_EQ_THM,DRESTRICT_DEF])
 
 val DRESTRICT_SUBSET = store_thm("DRESTRICT_SUBSET",
-  ``∀f1 f2 s t.
-    (DRESTRICT f1 s = DRESTRICT f2 s) ∧ t ⊆ s ⇒
+  ``!f1 f2 s t.
+    (DRESTRICT f1 s = DRESTRICT f2 s) /\ t SUBSET s ==>
     (DRESTRICT f1 t = DRESTRICT f2 t)``,
   rw[DRESTRICT_EQ_DRESTRICT]
     >- metis_tac[DRESTRICT_SUBSET_SUBMAP,SUBMAP_TRANS]
@@ -2582,7 +2583,7 @@ val DRESTRICT_SUBSET = store_thm("DRESTRICT_SUBSET",
   metis_tac[])
 
 val f_o_f_FUPDATE_compose = store_thm("f_o_f_FUPDATE_compose",
-  ``∀f1 f2 k x v. x ∉ FDOM f1 ∧ x ∉ FRANGE f2 ⇒
+  ``!f1 f2 k x v. x NOTIN FDOM f1 /\ x NOTIN FRANGE f2 ==>
     (f1 |+ (x,v) f_o_f f2 |+ (k,x) = (f1 f_o_f f2) |+ (k,v))``,
   rw[GSYM fmap_EQ_THM,f_o_f_DEF,FAPPLY_FUPDATE_THM] >>
   simp[] >> rw[] >> fs[] >> rw[EXTENSION] >>
@@ -2590,7 +2591,7 @@ val f_o_f_FUPDATE_compose = store_thm("f_o_f_FUPDATE_compose",
   >- PROVE_TAC[]
   >- PROVE_TAC[] >>
   qmatch_assum_rename_tac`y <> k`[] >>
-  `y ∈ FDOM (f1 f_o_f f2)` by rw[f_o_f_DEF] >>
+  `y IN FDOM (f1 f_o_f f2)` by rw[f_o_f_DEF] >>
   rw[f_o_f_DEF])
 
 val fmap_rel_trans = store_thm("fmap_rel_trans",
@@ -2610,18 +2611,18 @@ val fmap_eq_flookup = Q.store_thm ("fmap_eq_flookup",
  eq_tac >>
  rw [EXTENSION]
  >- metis_tac [NOT_SOME_NONE]
- >- (Cases_on `x ∉ FDOM m2` >>
+ >- (Cases_on `x NOTIN FDOM m2` >>
      fs []
      >- metis_tac [NOT_SOME_NONE]
      >- metis_tac [SOME_11]));
 
 val fupdate_list_map = Q.store_thm ("fupdate_list_map",
 `!l f x y.
-  x ∈ FDOM (FEMPTY |++ l)
-   ⇒
+  x IN FDOM (FEMPTY |++ l)
+   ==>
      ((FEMPTY |++ MAP (\(a,b). (a, f b)) l) ' x = f ((FEMPTY |++ l) ' x))`,
      rpt gen_tac >>
-     Q.ISPECL_THEN[`FST`,`f o SND`,`l`,`FEMPTY:α|->γ`]mp_tac(GSYM FOLDL_FUPDATE_LIST) >>
+     Q.ISPECL_THEN[`FST`,`f o SND`,`l`,`FEMPTY:'a|->'c`]mp_tac(GSYM FOLDL_FUPDATE_LIST) >>
      simp[LAMBDA_PROD] >>
      disch_then kall_tac >>
      qid_spec_tac`l` >>
@@ -2631,39 +2632,39 @@ val fupdate_list_map = Q.store_thm ("fupdate_list_map",
      rw[] >> rw[])
 
 val fdom_fupdate_list2 = Q.store_thm ("fdom_fupdate_list2",
-`∀kvl fm. FDOM (fm |++ kvl) = (FDOM fm DIFF set (MAP FST kvl)) ∪ set (MAP FST kvl)`,
+`!kvl fm. FDOM (fm |++ kvl) = (FDOM fm DIFF set (MAP FST kvl)) UNION set (MAP FST kvl)`,
 rw [FDOM_FUPDATE_LIST, EXTENSION] >>
 metis_tac []);
 
 val flookup_thm = Q.store_thm ("flookup_thm",
-`!f x v. ((FLOOKUP f x = NONE) = (x ∉ FDOM f)) ∧
-         ((FLOOKUP f x = SOME v) = (x ∈ FDOM f ∧ (f ' x = v)))`,
+`!f x v. ((FLOOKUP f x = NONE) = (x NOTIN FDOM f)) /\
+         ((FLOOKUP f x = SOME v) = (x IN FDOM f /\ (f ' x = v)))`,
 rw [FLOOKUP_DEF]);
 
 val FUPDATE_EQ_FUPDATE_LIST = store_thm("FUPDATE_EQ_FUPDATE_LIST",
-  ``∀fm kv. fm |+ kv = fm |++ [kv]``,
+  ``!fm kv. fm |+ kv = fm |++ [kv]``,
   rw[FUPDATE_LIST_THM]);
 
 val fmap_inverse_def = Define `
 fmap_inverse m1 m2 =
-  !k. k ∈ FDOM m1 ⇒ ?v. (FLOOKUP m1 k = SOME v) ∧ (FLOOKUP m2 v = SOME k)`;
+  !k. k IN FDOM m1 ==> ?v. (FLOOKUP m1 k = SOME v) /\ (FLOOKUP m2 v = SOME k)`;
 
 val fupdate_list_foldr = Q.store_thm ("fupdate_list_foldr",
-`!m l. FOLDR (λ(k,v) env. env |+ (k,v)) m l = m |++ REVERSE l`,
+`!m l. FOLDR (\(k,v) env. env |+ (k,v)) m l = m |++ REVERSE l`,
  Induct_on `l` >>
  rw [FUPDATE_LIST] >>
  PairCases_on `h` >>
  rw [FOLDL_APPEND]);
 
 val fupdate_list_foldl = Q.store_thm ("fupdate_list_foldl",
-`!m l. FOLDL (λenv (k,v). env |+ (k,v)) m l = m |++ l`,
+`!m l. FOLDL (\env (k,v). env |+ (k,v)) m l = m |++ l`,
  Induct_on `l` >>
  rw [FUPDATE_LIST] >>
  PairCases_on `h` >>
  rw []);
 
 val fmap_to_list = Q.store_thm ("fmap_to_list",
-`!m. ?l. ALL_DISTINCT (MAP FST l) ∧ (m = FEMPTY |++ l)`,
+`!m. ?l. ALL_DISTINCT (MAP FST l) /\ (m = FEMPTY |++ l)`,
 ho_match_mp_tac fmap_INDUCT >>
 rw [FUPDATE_LIST_THM] >|
 [qexists_tac `[]` >>
@@ -2674,11 +2675,11 @@ rw [FUPDATE_LIST_THM] >|
      rw [FUPDATE_FUPDATE_LIST_COMMUTES] >>
      fs [LIST_TO_SET_MAP] >>
      metis_tac [FST]]);
-     
+
 val disjoint_drestrict = Q.store_thm ("disjoint_drestrict",
-`!s m. DISJOINT s (FDOM m) ⇒ (DRESTRICT m (COMPL s) = m)`,
+`!s m. DISJOINT s (FDOM m) ==> (DRESTRICT m (COMPL s) = m)`,
  rw [fmap_eq_flookup, FLOOKUP_DRESTRICT] >>
- Cases_on `k ∉ s` >>
+ Cases_on `k NOTIN s` >>
  rw [] >>
  fs [DISJOINT_DEF, EXTENSION, FLOOKUP_DEF] >>
  metis_tac []);
@@ -2692,7 +2693,7 @@ val drestrict_iter_list = Q.store_thm ("drestrict_iter_list",
  metis_tac []);
 
 val fevery_funion = Q.store_thm ("fevery_funion",
-`!P m1 m2. FEVERY P m1 ∧ FEVERY P m2 ⇒ FEVERY P (FUNION m1 m2)`,
+`!P m1 m2. FEVERY P m1 /\ FEVERY P m2 ==> FEVERY P (FUNION m1 m2)`,
  rw [FEVERY_ALL_FLOOKUP, FLOOKUP_FUNION] >>
  BasicProvers.EVERY_CASE_TAC >>
  fs []);
@@ -2710,7 +2711,7 @@ val FUPDATE_LIST_ALL_DISTINCT_PERM = store_thm("FUPDATE_LIST_ALL_DISTINCT_PERM",
   qexists_tac `(fm |++ (M ++ N)) |+ (h0,h1)` >>
   conj_tac >- metis_tac[ALL_DISTINCT_PERM,PERM_MAP] >>
   rw[FUPDATE_LIST_APPEND] >>
-  `h0 ∉ set (MAP FST N)` by metis_tac[PERM_MEM_EQ,MEM_MAP,MEM_APPEND] >>
+  `h0 NOTIN set (MAP FST N)` by metis_tac[PERM_MEM_EQ,MEM_MAP,MEM_APPEND] >>
   imp_res_tac FUPDATE_FUPDATE_LIST_COMMUTES >>
   rw[FUPDATE_LIST_THM]);
 
